theories/common.v
@@ -1,4 +1,4 @@
-Require Import Autosubst2.unscoped Autosubst2.syntax Autosubst2.core ssreflect.
+Require Import Autosubst2.unscoped Autosubst2.syntax Autosubst2.core ssreflect ssrbool.
 From Equations Require Import Equations.
 Derive NoConfusion for nat PTag BTag PTm.
 Derive EqDec for BTag PTag PTm.
@@ -6,6 +6,7 @@ From Ltac2 Require Ltac2.
 Import Ltac2.Notations.
 Import Ltac2.Control.
 From Hammer Require Import Tactics.
+From stdpp Require Import relations (rtc(..)).
 
 Inductive lookup : nat -> list PTm -> PTm -> Prop :=
 | here A Γ : lookup 0 (cons A Γ) (ren_PTm shift A)
@@ -119,6 +120,28 @@ Definition isabs (a : PTm) :=
   | _ => false
   end.
 
+Definition tm_nonconf (a b : PTm) : bool :=
+  match a, b with
+  | PAbs _, _ => (~~ ishf b) || isabs b
+  | _, PAbs _ => ~~ ishf a
+  | VarPTm _, VarPTm _ => true
+  | PPair _ _, _ => (~~ ishf b) || ispair b
+  | _, PPair _ _ => ~~ ishf a
+  | PZero, PZero => true
+  | PSuc _, PSuc _ => true
+  | PApp _ _, PApp _ _ => (~~ ishf a) && (~~ ishf b)
+  | PProj _ _, PProj _ _ => (~~ ishf a) && (~~ ishf b)
+  | PInd _ _ _ _, PInd _ _ _ _ => (~~ ishf a) && (~~ ishf b)
+  | PNat, PNat => true
+  | PUniv _, PUniv _ => true
+  | PBind _ _ _, PBind _ _ _ => true
+  | _,_=> false
+  end.
+
+Definition tm_conf (a b : PTm) := ~~ tm_nonconf a b.
+
+
+
 Definition ishf_ren (a : PTm)  (ξ : nat -> nat) :
   ishf (ren_PTm ξ a) = ishf a.
 Proof. case : a => //=. Qed.
@@ -175,3 +198,390 @@ Module HRed.
 
     Definition nf a := forall b, ~ R a b.
 End HRed.
+
+Inductive algo_dom : PTm -> PTm -> Prop :=
+| A_AbsAbs a b :
+  algo_dom_r a b ->
+  (* --------------------- *)
+  algo_dom (PAbs a) (PAbs b)
+
+| A_AbsNeu a u :
+  ishne u ->
+  algo_dom_r a (PApp (ren_PTm shift u) (VarPTm var_zero)) ->
+  (* --------------------- *)
+  algo_dom (PAbs a) u
+
+| A_NeuAbs a u :
+  ishne u ->
+  algo_dom_r (PApp (ren_PTm shift u) (VarPTm var_zero)) a ->
+  (* --------------------- *)
+  algo_dom u (PAbs a)
+
+| A_PairPair a0 a1 b0 b1 :
+  algo_dom_r a0 a1 ->
+  algo_dom_r b0 b1 ->
+  (* ---------------------------- *)
+  algo_dom (PPair a0 b0) (PPair a1 b1)
+
+| A_PairNeu a0 a1 u :
+  ishne u ->
+  algo_dom_r a0 (PProj PL u) ->
+  algo_dom_r a1 (PProj PR u) ->
+  (* ----------------------- *)
+  algo_dom (PPair a0 a1) u
+
+| A_NeuPair a0 a1 u :
+  ishne u ->
+  algo_dom_r (PProj PL u) a0 ->
+  algo_dom_r (PProj PR u) a1 ->
+  (* ----------------------- *)
+  algo_dom u (PPair a0 a1)
+
+| A_ZeroZero :
+  algo_dom PZero PZero
+
+| A_SucSuc a0 a1 :
+  algo_dom_r a0 a1 ->
+  algo_dom (PSuc a0) (PSuc a1)
+
+| A_UnivCong i j :
+  (* -------------------------- *)
+  algo_dom (PUniv i) (PUniv j)
+
+| A_BindCong p0 p1 A0 A1 B0 B1 :
+  algo_dom_r A0 A1 ->
+  algo_dom_r B0 B1 ->
+  (* ---------------------------- *)
+  algo_dom (PBind p0 A0 B0) (PBind p1 A1 B1)
+
+| A_NatCong :
+  algo_dom PNat PNat
+
+| A_NeuNeu a b :
+  algo_dom_neu a b ->
+  algo_dom a b
+
+| A_Conf a b :
+  HRed.nf a ->
+  HRed.nf b ->
+  tm_conf a b ->
+  algo_dom a b
+
+with algo_dom_neu : PTm -> PTm -> Prop :=
+| A_VarCong i j :
+  (* -------------------------- *)
+  algo_dom_neu (VarPTm i) (VarPTm j)
+
+| A_AppCong u0 u1 a0 a1 :
+  ishne u0 ->
+  ishne u1 ->
+  algo_dom_neu u0 u1 ->
+  algo_dom_r a0 a1 ->
+  (* ------------------------- *)
+  algo_dom_neu (PApp u0 a0) (PApp u1 a1)
+
+| A_ProjCong p0 p1 u0 u1 :
+  ishne u0 ->
+  ishne u1 ->
+  algo_dom_neu u0 u1 ->
+  (* ---------------------  *)
+  algo_dom_neu (PProj p0 u0) (PProj p1 u1)
+
+| A_IndCong P0 P1 u0 u1 b0 b1 c0 c1 :
+  ishne u0 ->
+  ishne u1 ->
+  algo_dom_r P0 P1 ->
+  algo_dom_neu u0 u1 ->
+  algo_dom_r b0 b1 ->
+  algo_dom_r c0 c1 ->
+  algo_dom_neu (PInd P0 u0 b0 c0) (PInd P1 u1 b1 c1)
+
+with algo_dom_r : PTm  -> PTm -> Prop :=
+| A_NfNf a b :
+  algo_dom a b ->
+  algo_dom_r a b
+
+| A_HRedL a a' b  :
+  HRed.R a a' ->
+  algo_dom_r a' b ->
+  (* ----------------------- *)
+  algo_dom_r a b
+
+| A_HRedR a b b'  :
+  HRed.nf a ->
+  HRed.R b b' ->
+  algo_dom_r a b' ->
+  (* ----------------------- *)
+  algo_dom_r a b.
+
+Scheme algo_ind := Induction for algo_dom Sort Prop
+  with algo_neu_ind := Induction for algo_dom_neu Sort Prop
+  with algor_ind := Induction for algo_dom_r Sort Prop.
+
+Combined Scheme algo_dom_mutual from algo_ind, algo_neu_ind, algor_ind.
+#[export]Hint Constructors algo_dom algo_dom_neu algo_dom_r : adom.
+
+Definition stm_nonconf a b :=
+  match a, b with
+  | PUniv _, PUniv _ => true
+  | PBind PPi _ _, PBind PPi _ _ => true
+  | PBind PSig _ _, PBind PSig _ _ => true
+  | PNat, PNat => true
+  | VarPTm _, VarPTm _ => true
+  | PApp _ _, PApp _ _ => (~~ ishf a) && (~~ ishf b)
+  | PProj _ _, PProj _ _ => (~~ ishf a) && (~~ ishf b)
+  | PInd _ _ _ _, PInd _ _ _ _ => (~~ ishf a) && (~~ ishf b)
+  | _, _ => false
+  end.
+
+Lemma stm_tm_nonconf a b :
+  stm_nonconf a b -> tm_nonconf a b.
+Proof. apply /implyP.
+       destruct a ,b =>//=; hauto lq:on inv:PTag, BTag.
+Qed.
+
+Definition stm_conf a b := ~~ stm_nonconf a b.
+
+Lemma tm_stm_conf a b :
+  tm_conf a b -> stm_conf a b.
+Proof.
+  rewrite /tm_conf /stm_conf.
+  apply /contra /stm_tm_nonconf.
+Qed.
+
+Inductive salgo_dom : PTm -> PTm -> Prop :=
+| S_UnivCong i j :
+  (* -------------------------- *)
+  salgo_dom (PUniv i) (PUniv j)
+
+| S_PiCong  A0 A1 B0 B1 :
+  salgo_dom_r A1 A0 ->
+  salgo_dom_r B0 B1 ->
+  (* ---------------------------- *)
+  salgo_dom (PBind PPi A0 B0) (PBind PPi A1 B1)
+
+| S_SigCong  A0 A1 B0 B1 :
+  salgo_dom_r A0 A1 ->
+  salgo_dom_r B0 B1 ->
+  (* ---------------------------- *)
+  salgo_dom (PBind PSig A0 B0) (PBind PSig A1 B1)
+
+| S_NatCong :
+  salgo_dom PNat PNat
+
+| S_NeuNeu a b :
+  algo_dom_neu a b ->
+  salgo_dom a b
+
+| S_Conf a b :
+  HRed.nf a ->
+  HRed.nf b ->
+  stm_conf a b ->
+  salgo_dom a b
+
+with salgo_dom_r : PTm -> PTm -> Prop :=
+| S_NfNf a b :
+  salgo_dom a b ->
+  salgo_dom_r a b
+
+| S_HRedL a a' b  :
+  HRed.R a a' ->
+  salgo_dom_r a' b ->
+  (* ----------------------- *)
+  salgo_dom_r a b
+
+| S_HRedR a b b'  :
+  HRed.nf a ->
+  HRed.R b b' ->
+  salgo_dom_r a b' ->
+  (* ----------------------- *)
+  salgo_dom_r a b.
+
+Lemma hf_no_hred (a b : PTm) :
+  ishf a ->
+  HRed.R a b ->
+  False.
+Proof. hauto l:on inv:HRed.R. Qed.
+
+Lemma hne_no_hred (a b : PTm) :
+  ishne a ->
+  HRed.R a b ->
+  False.
+Proof. elim : a b => //=; hauto l:on inv:HRed.R. Qed.
+
+Ltac2 destruct_salgo () :=
+  lazy_match! goal with
+  | [h : is_true (ishne ?a) |- is_true (stm_conf ?a _) ] =>
+      if Constr.is_var a then destruct $a; ltac1:(done) else ()
+  | [|- is_true (stm_conf _ _)] =>
+      unfold stm_conf; ltac1:(done)
+  end.
+
+Ltac destruct_salgo := ltac2:(destruct_salgo ()).
+
+Lemma algo_dom_r_inv a b :
+  algo_dom_r a b -> exists a0 b0, algo_dom a0 b0 /\ rtc HRed.R a a0 /\ rtc HRed.R b b0.
+Proof.
+  induction 1; hauto lq:on ctrs:rtc.
+Qed.
+
+Lemma A_HRedsL a a' b :
+  rtc HRed.R a a' ->
+  algo_dom_r a' b ->
+  algo_dom_r a b.
+  induction 1; sfirstorder use:A_HRedL.
+Qed.
+
+Lemma A_HRedsR a b b' :
+  HRed.nf a ->
+  rtc HRed.R b b' ->
+  algo_dom a b' ->
+  algo_dom_r a b.
+Proof. induction 2; sauto. Qed.
+
+Lemma tm_conf_sym a b : tm_conf a b = tm_conf b a.
+Proof. case : a; case : b => //=. Qed.
+
+Lemma algo_dom_neu_hne (a b : PTm) :
+  algo_dom_neu a b ->
+  ishne a /\ ishne b.
+Proof. inversion 1; subst => //=. Qed.
+
+Lemma algo_dom_no_hred (a b : PTm) :
+  algo_dom a b ->
+  HRed.nf a /\ HRed.nf b.
+Proof.
+  induction 1 =>//=; try hauto inv:HRed.R use:hne_no_hred, hf_no_hred use:algo_dom_neu_hne lq:on unfold:HRed.nf.
+Qed.
+
+
+Lemma A_HRedR' a b b' :
+  HRed.R b b' ->
+  algo_dom_r a b' ->
+  algo_dom_r a b.
+Proof.
+  move => hb /algo_dom_r_inv.
+  move => [a0 [b0 [h0 [h1 h2]]]].
+  have {h2} {}hb : rtc HRed.R b b0 by hauto lq:on ctrs:rtc.
+  have ? : HRed.nf a0 by sfirstorder use:algo_dom_no_hred.
+  hauto lq:on use:A_HRedsL, A_HRedsR.
+Qed.
+
+Lemma algo_dom_sym :
+  (forall a b (h : algo_dom a b), algo_dom b a) /\
+    (forall a b, algo_dom_neu a b -> algo_dom_neu b a) /\
+    (forall a b (h : algo_dom_r a b), algo_dom_r b a).
+Proof.
+  apply algo_dom_mutual; try qauto use:tm_conf_sym,A_HRedR' db:adom.
+Qed.
+
+Lemma salgo_dom_r_inv a b :
+  salgo_dom_r a b -> exists a0 b0, salgo_dom a0 b0 /\ rtc HRed.R a a0 /\ rtc HRed.R b b0.
+Proof.
+  induction 1; hauto lq:on ctrs:rtc.
+Qed.
+
+Lemma S_HRedsL a a' b :
+  rtc HRed.R a a' ->
+  salgo_dom_r a' b ->
+  salgo_dom_r a b.
+  induction 1; sfirstorder use:S_HRedL.
+Qed.
+
+Lemma S_HRedsR a b b' :
+  HRed.nf a ->
+  rtc HRed.R b b' ->
+  salgo_dom a b' ->
+  salgo_dom_r a b.
+Proof. induction 2; sauto. Qed.
+
+Lemma stm_conf_sym a b : stm_conf a b = stm_conf b a.
+Proof. case : a; case : b => //=; hauto lq:on inv:PTag, BTag. Qed.
+
+Lemma salgo_dom_no_hred (a b : PTm) :
+  salgo_dom a b ->
+  HRed.nf a /\ HRed.nf b.
+Proof.
+  induction 1 =>//=; try hauto inv:HRed.R use:hne_no_hred, hf_no_hred, algo_dom_neu_hne lq:on unfold:HRed.nf.
+Qed.
+
+Lemma S_HRedR' a b b' :
+  HRed.R b b' ->
+  salgo_dom_r a b' ->
+  salgo_dom_r a b.
+Proof.
+  move => hb /salgo_dom_r_inv.
+  move => [a0 [b0 [h0 [h1 h2]]]].
+  have {h2} {}hb : rtc HRed.R b b0 by hauto lq:on ctrs:rtc.
+  have ? : HRed.nf a0 by sfirstorder use:salgo_dom_no_hred.
+  hauto lq:on use:S_HRedsL, S_HRedsR.
+Qed.
+
+Lemma algo_dom_salgo_dom :
+  (forall a b, algo_dom a b -> salgo_dom a b /\ salgo_dom b a) /\
+    (forall a b, algo_dom_neu a b -> True) /\
+    (forall a b, algo_dom_r a b -> salgo_dom_r a b /\ salgo_dom_r b a).
+Proof.
+  apply algo_dom_mutual => //=;
+                             try hauto lq:on ctrs:salgo_dom, algo_dom_neu, salgo_dom_r use:S_Conf, hne_no_hred, algo_dom_sym, tm_stm_conf, S_HRedR' inv:HRed.R unfold:HRed.nf  solve+:destruct_salgo.
+  - case;case; hauto lq:on ctrs:salgo_dom, algo_dom_neu, salgo_dom_r use:S_Conf, hne_no_hred, algo_dom_sym inv:HRed.R unfold:HRed.nf  solve+:destruct_salgo.
+  - move => a b ha hb /[dup] /tm_stm_conf h.
+    rewrite tm_conf_sym => /tm_stm_conf h0.
+    hauto l:on use:S_Conf inv:HRed.R unfold:HRed.nf.
+Qed.
+
+Fixpoint hred (a : PTm) : option (PTm) :=
+    match a with
+    | VarPTm i => None
+    | PAbs a => None
+    | PApp (PAbs a) b => Some (subst_PTm (scons b VarPTm) a)
+    | PApp a b =>
+        match hred a with
+        | Some a => Some (PApp a b)
+        | None => None
+        end
+    | PPair a b => None
+    | PProj p (PPair a b) => if p is PL then Some a else Some b
+    | PProj p a =>
+        match hred a with
+        | Some a => Some (PProj p a)
+        | None => None
+        end
+    | PUniv i => None
+    | PBind p A B => None
+    | PNat => None
+    | PZero => None
+    | PSuc a => None
+    | PInd P PZero b c => Some b
+    | PInd P (PSuc a) b c =>
+        Some (subst_PTm (scons (PInd P a b c) (scons a VarPTm)) c)
+    | PInd P a b c =>
+        match hred a with
+        | Some a => Some (PInd P a b c)
+        | None => None
+        end
+    end.
+
+Lemma hred_complete (a b : PTm) :
+  HRed.R a b -> hred a = Some b.
+Proof.
+  induction 1; hauto lq:on rew:off inv:HRed.R b:on.
+Qed.
+
+Lemma hred_sound (a b : PTm):
+  hred a = Some b -> HRed.R a b.
+Proof.
+  elim : a b; hauto q:on dep:on ctrs:HRed.R.
+Qed.
+
+Lemma hred_deter (a b0 b1 : PTm) :
+  HRed.R a b0 -> HRed.R a b1 -> b0 = b1.
+Proof.
+  move /hred_complete => + /hred_complete. congruence.
+Qed.
+
+Definition fancy_hred (a : PTm) : HRed.nf a + {b | HRed.R a b}.
+  destruct (hred a) eqn:eq.
+  right. exists p. by apply hred_sound in eq.
+  left. move => b /hred_complete. congruence.
+Defined.
